src/Parquet/cpp/EverParquet.h
@@ -925,11 +925,19 @@ Parquet_Pulse_Toplevel0_validate_footer(Pulse_Lib_Slice_slice__uint8_t uu___, si
 extern Parquet_Pulse_Toplevel_file_meta_data
 Parquet_Pulse_Toplevel0_read_footer(Pulse_Lib_Slice_slice__uint8_t uu___);
 
+bool Parquet_Pulse_Toplevel0_impl_validate_row_group_aux(Parquet_Pulse_Toplevel_row_group rg);
+
 FStar_Pervasives_Native_option__int64_t
 Parquet_Pulse_Toplevel0_compute_cols_size(
   bool *poverflow,
   Parquet_Pulse_Vec_vec__Parquet_Pulse_Toplevel_column_chunk cc,
   int64_t bound
+);
+
+bool
+Parquet_Pulse_Toplevel0_impl_validate_file_meta_data_aux(
+  int64_t data_size,
+  Parquet_Pulse_Toplevel_file_meta_data md
 );
 
 bool
